Preservation 20/52

ott_coq/destination_calculus_ott.v
@@ -58,13 +58,13 @@ Definition mode : Type := option (mul * age).
 Inductive term : Type :=  (*r Term *)
  | term_Val (v:val) (*r Value *)
  | term_Var (x:var) (*r Variable *)
- | term_App (t:term) (u:term) (*r Application *)
+ | term_App (t:term) (t':term) (*r Application *)
  | term_PatU (t:term) (u:term) (*r Pattern-match on unit *)
  | term_PatS (t:term) (m:mode) (x1:var) (u1:term) (x2:var) (u2:term) (*r Pattern-match on sum *)
  | term_PatP (t:term) (m:mode) (x1:var) (x2:var) (u:term) (*r Pattern-match on product *)
  | term_PatE (t:term) (m:mode) (n:mode) (x:var) (u:term) (*r Pattern-match on exponential *)
- | term_Map (t:term) (x:var) (u:term) (*r Map over the right side of ampar $(t:term)$ *)
- | term_ToA (t:term) (*r Wrap $(t:term)$ into a trivial ampar *)
+ | term_Map (t:term) (x:var) (t':term) (*r Map over the right side of ampar $(t:term)$ *)
+ | term_ToA (u:term) (*r Wrap $(u:term)$ into a trivial ampar *)
  | term_FromA (t:term) (*r Extract value from trivial ampar *)
  | term_Alloc : term (*r Return a fresh "identity" ampar object *)
  | term_FillU (t:term) (*r Fill destination with unit *)
@@ -73,26 +73,26 @@ Inductive term : Type :=  (*r Term *)
  | term_FillE (t:term) (m:mode) (*r Fill destination with exponential constructor *)
  | term_FillP (t:term) (*r Fill destination with product constructor *)
  | term_FillF (t:term) (x:var) (m:mode) (u:term) (*r Fill destination with function *)
- | term_FillC (t:term) (u:term) (*r Fill destination with root of ampar $(u:term)$ *)
+ | term_FillC (t:term) (t':term) (*r Fill destination with root of ampar $(t':term)$ *)
 with val : Type :=  (*r Term value *)
  | val_H (h:hdn) (*r Hole *)
  | val_D (h:hdn) (*r Destination *)
  | val_U : val (*r Unit *)
- | val_F (x:var) (m:mode) (t:term) (*r Lambda abstraction *)
+ | val_F (x:var) (m:mode) (u:term) (*r Lambda abstraction *)
  | val_L (v:val) (*r Left variant for sum *)
  | val_R (v:val) (*r Right variant for sum *)
  | val_E (m:mode) (v:val) (*r Exponential *)
  | val_P (v1:val) (v2:val) (*r Product *)
- | val_A (H:hdns) (v1:val) (v2:val) (*r Ampar *).
+ | val_A (H:hdns) (v2:val) (v1:val) (*r Ampar *).
 
 Inductive ectx : Type :=  (*r Evaluation context component *)
- | ectx_AppFoc1 (u:term) (*r Application *)
+ | ectx_AppFoc1 (t':term) (*r Application *)
  | ectx_AppFoc2 (v:val) (*r Application *)
  | ectx_PatUFoc (u:term) (*r Pattern-match on unit *)
  | ectx_PatSFoc (m:mode) (x1:var) (u1:term) (x2:var) (u2:term) (*r Pattern-match on sum *)
  | ectx_PatPFoc (m:mode) (x1:var) (x2:var) (u:term) (*r Pattern-match on product *)
  | ectx_PatEFoc (m:mode) (n:mode) (x:var) (u:term) (*r Pattern-match on exponential *)
- | ectx_MapFoc (x:var) (u:term) (*r Map over the right side of ampar *)
+ | ectx_MapFoc (x:var) (t':term) (*r Map over the right side of ampar *)
  | ectx_ToAFoc : ectx (*r Wrap into a trivial ampar *)
  | ectx_FromAFoc : ectx (*r Extract value from trivial ampar *)
  | ectx_FillUFoc : ectx (*r Fill destination with unit *)
@@ -101,17 +101,17 @@ Inductive ectx : Type :=  (*r Evaluation context component *)
  | ectx_FillEFoc (m:mode) (*r Fill destination with exponential constructor *)
  | ectx_FillPFoc : ectx (*r Fill destination with product constructor *)
  | ectx_FillFFoc (x:var) (m:mode) (u:term) (*r Fill destination with function *)
- | ectx_FillCFoc1 (u:term) (*r Fill destination with root of ampar *)
+ | ectx_FillCFoc1 (t':term) (*r Fill destination with root of ampar *)
  | ectx_FillCFoc2 (v:val) (*r Fill destination with root of ampar *)
- | ectx_AOpenFoc (H:hdns) (v1:val) (*r Open ampar. \textcolor{red}{Only new addition to term shapes} *).
+ | ectx_AOpenFoc (H:hdns) (v2:val) (*r Open ampar. \textcolor{red}{Only new addition to term shapes} *).
 
 Inductive type : Type :=  (*r Type *)
  | type_U : type (*r Unit *)
  | type_S (T1:type) (T2:type) (*r Sum *)
  | type_P (T1:type) (T2:type) (*r Product *)
  | type_E (m:mode) (T:type) (*r Exponential *)
- | type_A (T1:type) (T2:type) (*r Ampar type (consuming $(T2:type)$ yields $(T1:type)$) *)
- | type_F (T1:type) (m1:mode) (T2:type) (*r Function *)
+ | type_A (U:type) (T:type) (*r Ampar type (consuming $(T:type)$ yields $(U:type)$) *)
+ | type_F (T:type) (m:mode) (U:type) (*r Function *)
  | type_D (T:type) (m:mode) (*r Destination *).
 
 Inductive name : Type := 
@@ -441,24 +441,24 @@ Inductive TyR_val : ctx -> val -> type -> Prop :=    (* defn TyR_val *)
      TyR_val G (val_D h) (type_D T n)
  | TyR_val_U : 
      TyR_val  ctx_empty  val_U type_U
- | TyR_val_F : forall (D:ctx) (x:var) (m:mode) (t:term) (T1 T2:type)
-     (Tyt: Ty_term  (ctx_union  D    (ctx_singleton (name_Var  x ) (tyb_Var  m   T1 ))  )  t T2),
+ | TyR_val_F : forall (D:ctx) (x:var) (m:mode) (u:term) (T U:type)
+     (Tyu: Ty_term  (ctx_union  D    (ctx_singleton (name_Var  x ) (tyb_Var  m   T ))  )  u U),
      ctx_DestOnly D  ->
-     TyR_val D (val_F x m t) (type_F T1 m T2)
- | TyR_val_L : forall (G:ctx) (v:val) (T1 T2:type)
-     (TyRv: TyR_val G v T1),
-     TyR_val G (val_L v) (type_S T1 T2)
- | TyR_val_R : forall (G:ctx) (v:val) (T1 T2:type)
-     (TyRv: TyR_val G v T2),
-     TyR_val G (val_R v) (type_S T1 T2)
+     TyR_val D (val_F x m u) (type_F T m U)
+ | TyR_val_L : forall (G:ctx) (v1:val) (T1 T2:type)
+     (TyRv1: TyR_val G v1 T1),
+     TyR_val G (val_L v1) (type_S T1 T2)
+ | TyR_val_R : forall (G:ctx) (v2:val) (T1 T2:type)
+     (TyRv2: TyR_val G v2 T2),
+     TyR_val G (val_R v2) (type_S T1 T2)
  | TyR_val_P : forall (G1 G2:ctx) (v1 v2:val) (T1 T2:type)
      (TyRv1: TyR_val G1 v1 T1)
      (TyRv2: TyR_val G2 v2 T2),
      TyR_val  (ctx_union  G1   G2 )  (val_P v1 v2) (type_P T1 T2)
- | TyR_val_E : forall (n:mode) (G:ctx) (v:val) (T:type)
-     (TyRv: TyR_val G v T),
-     TyR_val  (ctx_stimes  n   G )  (val_E n v) (type_E n T)
- | TyR_val_A : forall (D1 D2 D3:ctx) (v1 v2:val) (T1 T2:type)
+ | TyR_val_E : forall (n:mode) (G:ctx) (v':val) (T:type)
+     (TyRvp: TyR_val G v' T),
+     TyR_val  (ctx_stimes  n   G )  (val_E n v') (type_E n T)
+ | TyR_val_A : forall (D1 D2 D3:ctx) (v2 v1:val) (U T:type)
      (DestOnlyD1: ctx_DestOnly D1 )
      (DestOnlyD2: ctx_DestOnly D2 )
      (DestOnlyD3: ctx_DestOnly D3 )
@@ -467,21 +467,21 @@ Inductive TyR_val : ctx -> val -> type -> Prop :=    (* defn TyR_val *)
      (DisjointD1D2: ctx_Disjoint D1 D2 )
      (DisjointD1D3: ctx_Disjoint D1 D3 )
      (DisjointD2D3: ctx_Disjoint D2 D3 )
-     (TyRv1: TyR_val  (ctx_union  D1     (ctx_minus  D3 )   )  v1 T1)
-     (TyRv2: TyR_val  (ctx_union  D2   D3 )  v2 T2),
-     TyR_val  (ctx_union  D1   D2 )  (val_A  (hdns_from_ctx   (ctx_minus  D3 )  )  v1 v2) (type_A T1 T2)
+     (TyRv1: TyR_val  (ctx_union  D1   D3 )  v1 T)
+     (TyRv2: TyR_val  (ctx_union  D2     (ctx_minus  D3 )   )  v2 U),
+     TyR_val  (ctx_union  D1   D2 )  (val_A  (hdns_from_ctx   (ctx_minus  D3 )  )  v2 v1) (type_A U T)
 with Ty_term : ctx -> term -> type -> Prop :=    (* defn Ty_term *)
- | Ty_term_Val : forall (D:ctx) (v:val) (T:type),
+ | Ty_term_Val : forall (D:ctx) (v:val) (T:type)
+     (TyRv: TyR_val D v T),
      ctx_DestOnly D  ->
-     TyR_val D v T ->
      Ty_term D (term_Val v) T
  | Ty_term_Var : forall (P:ctx) (x:var) (T:type)
      (CompatPx: ctx_CompatibleVar P x (tyb_Var  (Some (pair   Lin     (Fin 0)  ))  T) ),
      Ty_term P (term_Var x) T
- | Ty_term_App : forall (m:mode) (P1 P2:ctx) (t u:term) (T2 T1:type)
-     (Tyt: Ty_term P1 t T1)
-     (Tyu: Ty_term P2 u (type_F T1 m T2)),
-     Ty_term  (ctx_union   (ctx_stimes  m   P1 )    P2 )  (term_App t u) T2
+ | Ty_term_App : forall (m:mode) (P1 P2:ctx) (t t':term) (U T:type)
+     (Tyt: Ty_term P1 t T)
+     (Tytp: Ty_term P2 t' (type_F T m U)),
+     Ty_term  (ctx_union   (ctx_stimes  m   P1 )    P2 )  (term_App t t') U
  | Ty_term_PatU : forall (P1 P2:ctx) (t u:term) (U:type)
      (Tyt: Ty_term P1 t type_U)
      (Tyu: Ty_term P2 u U),
@@ -505,19 +505,19 @@ with Ty_term : ctx -> term -> type -> Prop :=    (* defn Ty_term *)
      (Tyt: Ty_term P1 t (type_E n T))
      (Tyu: Ty_term  (ctx_union  P2    (ctx_singleton (name_Var  x ) (tyb_Var   (mode_times'  ((app (cons m nil) (app (cons n nil) nil))) )    T ))  )  u U),
      Ty_term  (ctx_union   (ctx_stimes  m   P1 )    P2 )  (term_PatE t m n x u) U
- | Ty_term_Map : forall (P1 P2:ctx) (t:term) (x:var) (u:term) (T1 U T2:type)
-     (DisjointP2x: ctx_Disjoint P2  (ctx_singleton (name_Var  x ) (tyb_Var   (Some (pair   Lin     (Fin 0)  ))    T2 ))  )
-     (Tyt: Ty_term P1 t (type_A T1 T2))
-     (Tyu: Ty_term  (ctx_union   (ctx_stimes   (Some (pair   Lin     (Fin 1)  ))    P2 )     (ctx_singleton (name_Var  x ) (tyb_Var   (Some (pair   Lin     (Fin 0)  ))    T2 ))  )  u U),
-     Ty_term  (ctx_union  P1   P2 )  (term_Map t x u) (type_A T1 U)
- | Ty_term_ToA : forall (P:ctx) (t:term) (T:type)
-     (Tyt: Ty_term P t T),
-     Ty_term P (term_ToA t) (type_A T type_U)
- | Ty_term_FromA : forall (P:ctx) (t:term) (T:type)
-     (Tyt: Ty_term P t (type_A T type_U)),
-     Ty_term P (term_FromA t) T
- | Ty_term_Alloc : forall (T:type),
-     Ty_term  ctx_empty  term_Alloc (type_A T (type_D T  (Some (pair   Lin     (Fin 0)  )) ))
+ | Ty_term_Map : forall (P1 P2:ctx) (t:term) (x:var) (t':term) (U T' T:type)
+     (DisjointP2x: ctx_Disjoint P2  (ctx_singleton (name_Var  x ) (tyb_Var   (Some (pair   Lin     (Fin 0)  ))    T ))  )
+     (Tyt: Ty_term P1 t (type_A U T))
+     (Tytp: Ty_term  (ctx_union   (ctx_stimes   (Some (pair   Lin     (Fin 1)  ))    P2 )     (ctx_singleton (name_Var  x ) (tyb_Var   (Some (pair   Lin     (Fin 0)  ))    T ))  )  t' T'),
+     Ty_term  (ctx_union  P1   P2 )  (term_Map t x t') (type_A U T')
+ | Ty_term_ToA : forall (P:ctx) (u:term) (U:type)
+     (Tyu: Ty_term P u U),
+     Ty_term P (term_ToA u) (type_A U type_U)
+ | Ty_term_FromA : forall (P:ctx) (t:term) (U:type)
+     (Tyt: Ty_term P t (type_A U type_U)),
+     Ty_term P (term_FromA t) U
+ | Ty_term_Alloc : forall (U:type),
+     Ty_term  ctx_empty  term_Alloc (type_A U (type_D U  (Some (pair   Lin     (Fin 0)  )) ))
  | Ty_term_FillU : forall (P:ctx) (t:term) (n:mode)
      (Tyt: Ty_term P t (type_D type_U n)),
      Ty_term P (term_FillU t) type_U
@@ -533,35 +533,35 @@ with Ty_term : ctx -> term -> type -> Prop :=    (* defn Ty_term *)
  | Ty_term_FillE : forall (P:ctx) (t:term) (n':mode) (T:type) (n:mode)
      (Tyt: Ty_term P t (type_D (type_E n' T) n)),
      Ty_term P (term_FillE t n') (type_D T  (mode_times'  ((app (cons n' nil) (app (cons n nil) nil))) ) )
- | Ty_term_FillF : forall (P1:ctx) (n:mode) (P2:ctx) (t:term) (x:var) (m:mode) (u:term) (T1 T2:type)
-     (DisjointP2x: ctx_Disjoint P2  (ctx_singleton (name_Var  x ) (tyb_Var  m   T1 ))  )
-     (Tyt: Ty_term P1 t (type_D (type_F T1 m T2) n))
-     (Tyu: Ty_term  (ctx_union  P2    (ctx_singleton (name_Var  x ) (tyb_Var  m   T1 ))  )  u T2),
+ | Ty_term_FillF : forall (P1:ctx) (n:mode) (P2:ctx) (t:term) (x:var) (m:mode) (u:term) (T U:type)
+     (DisjointP2x: ctx_Disjoint P2  (ctx_singleton (name_Var  x ) (tyb_Var  m   T ))  )
+     (Tyt: Ty_term P1 t (type_D (type_F T m U) n))
+     (Tyu: Ty_term  (ctx_union  P2    (ctx_singleton (name_Var  x ) (tyb_Var  m   T ))  )  u U),
      Ty_term  (ctx_union  P1    (ctx_stimes    (mode_times'  ((app (cons  (Some (pair   Lin     (Fin 1)  ))  nil) (app (cons n nil) nil))) )     P2 )  )  (term_FillF t x m u) type_U
- | Ty_term_FillC : forall (P1:ctx) (n:mode) (P2:ctx) (t u:term) (T2 T1:type)
-     (Tyt: Ty_term P1 t (type_D T1 n))
-     (Tyu: Ty_term P2 u (type_A T1 T2)),
-     Ty_term  (ctx_union  P1    (ctx_stimes    (mode_times'  ((app (cons  (Some (pair   Lin     (Fin 1)  ))  nil) (app (cons n nil) nil))) )     P2 )  )  (term_FillC t u) T2
+ | Ty_term_FillC : forall (P1:ctx) (n:mode) (P2:ctx) (t t':term) (T U:type)
+     (Tyt: Ty_term P1 t (type_D U n))
+     (Tytp: Ty_term P2 t' (type_A U T)),
+     Ty_term  (ctx_union  P1    (ctx_stimes    (mode_times'  ((app (cons  (Some (pair   Lin     (Fin 1)  ))  nil) (app (cons n nil) nil))) )     P2 )  )  (term_FillC t t') T
 with Ty_ectxs : ctx -> ectxs -> type -> type -> Prop :=    (* defn Ty_ectxs *)
  | Ty_ectxs_Id : forall (U0:type),
      Ty_ectxs  ctx_empty   nil  U0 U0
- | Ty_ectxs_AppFoc1 : forall (D1:ctx) (C:ectxs) (u:term) (T1 U0:type) (D2:ctx) (m:mode) (T2:type)
+ | Ty_ectxs_AppFoc1 : forall (D1:ctx) (C:ectxs) (t':term) (T U0:type) (D2:ctx) (m:mode) (U:type)
      (DisjointD1D2: ctx_Disjoint D1 D2 )
      (DestOnlyD1: ctx_DestOnly D1 )
      (DestOnlyD2: ctx_DestOnly D2 )
      (Validm: mode_IsValid m )
      (ValidOnlyD2: ctx_ValidOnly D2 )
-     (TyC: Ty_ectxs  (ctx_union   (ctx_stimes  m   D1 )    D2 )  C T2 U0)
-     (Tyu: Ty_term D2 u (type_F T1 m T2)),
-     Ty_ectxs D1  (cons   (ectx_AppFoc1 u)    C )  T1 U0
- | Ty_ectxs_AppFoc2 : forall (D2:ctx) (C:ectxs) (v:val) (T1:type) (m:mode) (T2 U0:type) (D1:ctx)
+     (TyC: Ty_ectxs  (ctx_union   (ctx_stimes  m   D1 )    D2 )  C U U0)
+     (Tytp: Ty_term D2 t' (type_F T m U)),
+     Ty_ectxs D1  (cons   (ectx_AppFoc1 t')    C )  T U0
+ | Ty_ectxs_AppFoc2 : forall (D2:ctx) (C:ectxs) (v:val) (T:type) (m:mode) (U U0:type) (D1:ctx)
      (DisjointD1D2: ctx_Disjoint D1 D2 )
      (DestOnlyD1: ctx_DestOnly D1 )
      (DestOnlyD2: ctx_DestOnly D2 )
      (ValidmD1: ctx_ValidOnly  (ctx_stimes  m   D1 )  )
-     (TyC: Ty_ectxs  (ctx_union   (ctx_stimes  m   D1 )    D2 )  C T2 U0)
-     (Tyv: Ty_term D1 (term_Val v) T1),
-     Ty_ectxs D2  (cons   (ectx_AppFoc2 v)    C )   (type_F T1 m T2)  U0
+     (TyC: Ty_ectxs  (ctx_union   (ctx_stimes  m   D1 )    D2 )  C U U0)
+     (Tyv: Ty_term D1 (term_Val v) T),
+     Ty_ectxs D2  (cons   (ectx_AppFoc2 v)    C )   (type_F T m U)  U0
  | Ty_ectxs_PatUFoc : forall (D1:ctx) (C:ectxs) (u:term) (U0:type) (D2:ctx) (U:type)
      (DisjointD1D2: ctx_Disjoint D1 D2 )
      (DestOnlyD1: ctx_DestOnly D1 )
@@ -599,20 +599,20 @@ with Ty_ectxs : ctx -> ectxs -> type -> type -> Prop :=    (* defn Ty_ectxs *)
      (TyC: Ty_ectxs  (ctx_union   (ctx_stimes  m   D1 )    D2 )  C U U0)
      (Tyu: Ty_term  (ctx_union  D2    (ctx_singleton (name_Var  x ) (tyb_Var   (mode_times'  ((app (cons m nil) (app (cons m' nil) nil))) )    T ))  )  u U),
      Ty_ectxs D1  (cons   (ectx_PatEFoc m m' x u)    C )  (type_E m' T) U0
- | Ty_ectxs_MapFoc : forall (D1:ctx) (C:ectxs) (x:var) (u:term) (T1 T2 U0:type) (D2:ctx) (U:type)
+ | Ty_ectxs_MapFoc : forall (D1:ctx) (C:ectxs) (x:var) (t':term) (U T U0:type) (D2:ctx) (T':type)
      (DisjointD1D2: ctx_Disjoint D1 D2 )
      (DestOnlyD1: ctx_DestOnly D1 )
      (DestOnlyD2: ctx_DestOnly D2 )
      (ValidOnlyD2: ctx_ValidOnly D2 )
-     (TyC: Ty_ectxs  (ctx_union  D1   D2 )  C U U0)
-     (Tyu: Ty_term  (ctx_union   (ctx_stimes   (Some (pair   Lin     (Fin 1)  ))    D2 )     (ctx_singleton (name_Var  x ) (tyb_Var   (Some (pair   Lin     (Fin 0)  ))    T2 ))  )  u U),
-     Ty_ectxs D1  (cons   (ectx_MapFoc x u)    C )   (type_A T1 T2)  U0
- | Ty_ectxs_ToAFoc : forall (D:ctx) (C:ectxs) (T U0:type)
-     (TyC: Ty_ectxs D C  (type_A T type_U)  U0),
-     Ty_ectxs D  (cons   ectx_ToAFoc    C )  T U0
- | Ty_ectxs_FromAFoc : forall (D:ctx) (C:ectxs) (T U0:type)
-     (TyC: Ty_ectxs D C T U0),
-     Ty_ectxs D  (cons   ectx_FromAFoc    C )   (type_A T type_U)  U0
+     (TyC: Ty_ectxs  (ctx_union  D1   D2 )  C (type_A U T') U0)
+     (Tytp: Ty_term  (ctx_union   (ctx_stimes   (Some (pair   Lin     (Fin 1)  ))    D2 )     (ctx_singleton (name_Var  x ) (tyb_Var   (Some (pair   Lin     (Fin 0)  ))    T ))  )  t' T'),
+     Ty_ectxs D1  (cons   (ectx_MapFoc x t')    C )   (type_A U T)  U0
+ | Ty_ectxs_ToAFoc : forall (D:ctx) (C:ectxs) (U U0:type)
+     (TyC: Ty_ectxs D C  (type_A U type_U)  U0),
+     Ty_ectxs D  (cons   ectx_ToAFoc    C )  U U0
+ | Ty_ectxs_FromAFoc : forall (D:ctx) (C:ectxs) (U U0:type)
+     (TyC: Ty_ectxs D C U U0),
+     Ty_ectxs D  (cons   ectx_FromAFoc    C )   (type_A U type_U)  U0
  | Ty_ectxs_FillUFoc : forall (D:ctx) (C:ectxs) (n:mode) (U0:type)
      (TyC: Ty_ectxs D C type_U U0),
      Ty_ectxs D  (cons   ectx_FillUFoc    C )  (type_D type_U n) U0
@@ -628,32 +628,32 @@ with Ty_ectxs : ctx -> ectxs -> type -> type -> Prop :=    (* defn Ty_ectxs *)
  | Ty_ectxs_FillEFoc : forall (D:ctx) (C:ectxs) (m:mode) (T:type) (n:mode) (U0:type)
      (TyC: Ty_ectxs D C (type_D T  (mode_times'  ((app (cons m nil) (app (cons n nil) nil))) ) ) U0),
      Ty_ectxs D  (cons   (ectx_FillEFoc m)    C )  (type_D (type_E m T) n) U0
- | Ty_ectxs_FillFFoc : forall (D1:ctx) (C:ectxs) (x:var) (m:mode) (u:term) (T1 T2:type) (n:mode) (U0:type) (D2:ctx)
+ | Ty_ectxs_FillFFoc : forall (D1:ctx) (C:ectxs) (x:var) (m:mode) (u:term) (T U:type) (n:mode) (U0:type) (D2:ctx)
      (DisjointD1D2: ctx_Disjoint D1 D2 )
      (DestOnlyD1: ctx_DestOnly D1 )
      (DestOnlyD2: ctx_DestOnly D2 )
      (ValidsnD2: ctx_ValidOnly  (ctx_stimes    (mode_times'  ((app (cons  (Some (pair   Lin     (Fin 1)  ))  nil) (app (cons n nil) nil))) )     D2 )  )
      (TyC: Ty_ectxs  (ctx_union  D1    (ctx_stimes    (mode_times'  ((app (cons  (Some (pair   Lin     (Fin 1)  ))  nil) (app (cons n nil) nil))) )     D2 )  )  C type_U U0)
-     (Tyu: Ty_term  (ctx_union  D2    (ctx_singleton (name_Var  x ) (tyb_Var  m   T1 ))  )  u T2),
-     Ty_ectxs D1  (cons   (ectx_FillFFoc x m u)    C )  (type_D (type_F T1 m T2) n) U0
- | Ty_ectxs_FillCFoc1 : forall (D1:ctx) (C:ectxs) (u:term) (T1:type) (n:mode) (U0:type) (D2:ctx) (T2:type)
+     (Tyu: Ty_term  (ctx_union  D2    (ctx_singleton (name_Var  x ) (tyb_Var  m   T ))  )  u U),
+     Ty_ectxs D1  (cons   (ectx_FillFFoc x m u)    C )  (type_D (type_F T m U) n) U0
+ | Ty_ectxs_FillCFoc1 : forall (D1:ctx) (C:ectxs) (t':term) (U:type) (n:mode) (U0:type) (D2:ctx) (T:type)
      (DisjointD1D2: ctx_Disjoint D1 D2 )
      (DestOnlyD1: ctx_DestOnly D1 )
      (DestOnlyD2: ctx_DestOnly D2 )
      (ValidsnD2: ctx_ValidOnly  (ctx_stimes    (mode_times'  ((app (cons  (Some (pair   Lin     (Fin 1)  ))  nil) (app (cons n nil) nil))) )     D2 )  )
-     (TyC: Ty_ectxs  (ctx_union  D1    (ctx_stimes    (mode_times'  ((app (cons  (Some (pair   Lin     (Fin 1)  ))  nil) (app (cons n nil) nil))) )     D2 )  )  C T2 U0)
-     (Tyu: Ty_term D2 u (type_A T1 T2)),
-     Ty_ectxs D1  (cons   (ectx_FillCFoc1 u)    C )  (type_D T1 n) U0
- | Ty_ectxs_FillCFoc2 : forall (D2:ctx) (C:ectxs) (v:val) (T1 T2 U0:type) (D1:ctx) (n:mode)
+     (TyC: Ty_ectxs  (ctx_union  D1    (ctx_stimes    (mode_times'  ((app (cons  (Some (pair   Lin     (Fin 1)  ))  nil) (app (cons n nil) nil))) )     D2 )  )  C T U0)
+     (Tytp: Ty_term D2 t' (type_A U T)),
+     Ty_ectxs D1  (cons   (ectx_FillCFoc1 t')    C )  (type_D U n) U0
+ | Ty_ectxs_FillCFoc2 : forall (D2:ctx) (C:ectxs) (v:val) (U T U0:type) (D1:ctx) (n:mode)
      (DisjointD1D2: ctx_Disjoint D1 D2 )
      (DestOnlyD1: ctx_DestOnly D1 )
      (DestOnlyD2: ctx_DestOnly D2 )
      (ValidsnD1: ctx_ValidOnly D1 )
      (Validsn: mode_IsValid   (mode_times'  ((app (cons  (Some (pair   Lin     (Fin 1)  ))  nil) (app (cons n nil) nil))) )   )
-     (TyC: Ty_ectxs  (ctx_union  D1    (ctx_stimes    (mode_times'  ((app (cons  (Some (pair   Lin     (Fin 1)  ))  nil) (app (cons n nil) nil))) )     D2 )  )  C T2 U0)
-     (Tyu: Ty_term D1 (term_Val v) (type_D T1 n)),
-     Ty_ectxs D2  (cons   (ectx_FillCFoc2 v)    C )  (type_A T1 T2) U0
- | Ty_ectxs_AOpenFoc : forall (D2 D3:ctx) (C:ectxs) (v1:val) (U U0:type) (D1:ctx) (T1:type)
+     (TyC: Ty_ectxs  (ctx_union  D1    (ctx_stimes    (mode_times'  ((app (cons  (Some (pair   Lin     (Fin 1)  ))  nil) (app (cons n nil) nil))) )     D2 )  )  C T U0)
+     (Tyt: Ty_term D1 (term_Val v) (type_D U n)),
+     Ty_ectxs D2  (cons   (ectx_FillCFoc2 v)    C )  (type_A U T) U0
+ | Ty_ectxs_AOpenFoc : forall (D1 D3:ctx) (C:ectxs) (v2:val) (T' U0:type) (D2:ctx) (U:type)
      (DisjoinD1D2: ctx_Disjoint D1 D2 )
      (DisjoinD1D3: ctx_Disjoint D1 D3 )
      (DestOnlyD1: ctx_DestOnly D1 )
@@ -661,10 +661,10 @@ with Ty_ectxs : ctx -> ectxs -> type -> type -> Prop :=    (* defn Ty_ectxs *)
      (DestOnlyD3: ctx_DestOnly D3 )
      (LinOnlyD3: ctx_LinOnly D3 )
      (ValidOnlyD1: ctx_ValidOnly D1 )
-     (TyC: Ty_ectxs  (ctx_union  D1   D2 )  C  (type_A T1 U)  U0)
-     (TyRv1: TyR_val  (ctx_union  D1    (ctx_minus  D3 )  )  v1 T1),
+     (TyC: Ty_ectxs  (ctx_union  D1   D2 )  C  (type_A U T')  U0)
+     (TyRv2: TyR_val  (ctx_union  D2    (ctx_minus  D3 )  )  v2 U),
      hdns_Disjoint  (hdns_from_ectxs  C )   (hdns_from_ctx   (ctx_minus  D3 )  )   ->
-     Ty_ectxs  (ctx_union   (ctx_stimes   (Some (pair   Lin     (Fin 1)  ))    D2 )    D3 )   (cons   (ectx_AOpenFoc  (hdns_from_ctx   (ctx_minus  D3 )  )  v1)    C )  U U0
+     Ty_ectxs  (ctx_union   (ctx_stimes   (Some (pair   Lin     (Fin 1)  ))    D1 )    D3 )   (cons   (ectx_AOpenFoc  (hdns_from_ctx   (ctx_minus  D3 )  )  v2)    C )  T' U0
 with Ty_eterm : ectxs -> term -> type -> Prop :=    (* defn Ty_eterm *)
  | Ty_eterm_ClosedEterm : forall (C:ectxs) (t:term) (U0:type) (D:ctx) (T:type)
      (ValidOnlyD: ctx_ValidOnly D )
@@ -676,18 +676,18 @@ with Ty_eterm : ectxs -> term -> type -> Prop :=    (* defn Ty_eterm *)
 
 (* defns Sem *)
 Inductive Sem_eterm : ectxs -> term -> ectxs -> term -> Prop :=    (* defn Sem_eterm *)
- | Sem_eterm_AppFoc1 : forall (C:ectxs) (t u:term)
+ | Sem_eterm_AppFoc1 : forall (C:ectxs) (t t':term)
      (NotValt: term_NotVal t ),
-     Sem_eterm C (term_App t u)   (cons   (ectx_AppFoc1 u)    C )   t
- | Sem_eterm_AppUnfoc1 : forall (C:ectxs) (u:term) (v:val),
-     Sem_eterm   (cons   (ectx_AppFoc1 u)    C )   (term_Val v) C (term_App (term_Val v) u)
- | Sem_eterm_AppFoc2 : forall (C:ectxs) (v:val) (u:term)
-     (NotValu: term_NotVal u ),
-     Sem_eterm C (term_App (term_Val v) u)   (cons   (ectx_AppFoc2 v)    C )   u
+     Sem_eterm C (term_App t t')   (cons   (ectx_AppFoc1 t')    C )   t
+ | Sem_eterm_AppUnfoc1 : forall (C:ectxs) (t':term) (v:val),
+     Sem_eterm   (cons   (ectx_AppFoc1 t')    C )   (term_Val v) C (term_App (term_Val v) t')
+ | Sem_eterm_AppFoc2 : forall (C:ectxs) (v:val) (t':term)
+     (NotValtp: term_NotVal t' ),
+     Sem_eterm C (term_App (term_Val v) t')   (cons   (ectx_AppFoc2 v)    C )   t'
  | Sem_eterm_AppUnfoc2 : forall (C:ectxs) (v v':val),
      Sem_eterm   (cons   (ectx_AppFoc2 v)    C )   (term_Val v') C (term_App (term_Val v) (term_Val v'))
- | Sem_eterm_AppRed : forall (C:ectxs) (v:val) (x:var) (m:mode) (t:term),
-     Sem_eterm C (term_App (term_Val v) (term_Val  (val_F x m t) )) C  (term_sub  t   x   v ) 
+ | Sem_eterm_AppRed : forall (C:ectxs) (v:val) (x:var) (m:mode) (u:term),
+     Sem_eterm C (term_App (term_Val v) (term_Val  (val_F x m u) )) C  (term_sub  u   x   v ) 
  | Sem_eterm_PatUFoc : forall (C:ectxs) (t u:term)
      (NotValt: term_NotVal t ),
      Sem_eterm C (term_PatU t u)   (cons   (ectx_PatUFoc u)    C )   t
@@ -700,10 +700,10 @@ Inductive Sem_eterm : ectxs -> term -> ectxs -> term -> Prop :=    (* defn Sem_e
      Sem_eterm C (term_PatS t m x1 u1 x2 u2)   (cons   (ectx_PatSFoc m x1 u1 x2 u2)    C )   t
  | Sem_eterm_PatSUnfoc : forall (C:ectxs) (m:mode) (x1:var) (u1:term) (x2:var) (u2:term) (v:val),
      Sem_eterm   (cons   (ectx_PatSFoc m x1 u1 x2 u2)    C )   (term_Val v) C (term_PatS (term_Val v) m x1 u1 x2 u2)
- | Sem_eterm_PatLRed : forall (C:ectxs) (v:val) (m:mode) (x1:var) (u1:term) (x2:var) (u2:term),
-     Sem_eterm C (term_PatS (term_Val  (val_L v) ) m x1 u1 x2 u2) C  (term_sub  u1   x1   v ) 
- | Sem_eterm_PatRRed : forall (C:ectxs) (v:val) (m:mode) (x1:var) (u1:term) (x2:var) (u2:term),
-     Sem_eterm C (term_PatS (term_Val  (val_R v) ) m x1 u1 x2 u2) C  (term_sub  u2   x2   v ) 
+ | Sem_eterm_PatLRed : forall (C:ectxs) (v1:val) (m:mode) (x1:var) (u1:term) (x2:var) (u2:term),
+     Sem_eterm C (term_PatS (term_Val  (val_L v1) ) m x1 u1 x2 u2) C  (term_sub  u1   x1   v1 ) 
+ | Sem_eterm_PatRRed : forall (C:ectxs) (v2:val) (m:mode) (x1:var) (u1:term) (x2:var) (u2:term),
+     Sem_eterm C (term_PatS (term_Val  (val_R v2) ) m x1 u1 x2 u2) C  (term_sub  u2   x2   v2 ) 
  | Sem_eterm_PatPFoc : forall (C:ectxs) (t:term) (m:mode) (x1 x2:var) (u:term)
      (NotValt: term_NotVal t ),
      Sem_eterm C (term_PatP t m x1 x2 u)   (cons   (ectx_PatPFoc m x1 x2 u)    C )   t
@@ -716,34 +716,34 @@ Inductive Sem_eterm : ectxs -> term -> ectxs -> term -> Prop :=    (* defn Sem_e
      Sem_eterm C (term_PatE t m n x u)   (cons   (ectx_PatEFoc m n x u)    C )   t
  | Sem_eterm_PatEUnfoc : forall (C:ectxs) (m n:mode) (x:var) (u:term) (v:val),
      Sem_eterm   (cons   (ectx_PatEFoc m n x u)    C )   (term_Val v) C (term_PatE (term_Val v) m n x u)
- | Sem_eterm_PatERed : forall (C:ectxs) (n:mode) (v:val) (m:mode) (x:var) (u:term),
-     Sem_eterm C (term_PatE (term_Val (val_E n v)) m n x u) C  (term_sub  u   x   v ) 
- | Sem_eterm_MapFoc : forall (C:ectxs) (t:term) (x:var) (u:term)
+ | Sem_eterm_PatERed : forall (C:ectxs) (n:mode) (v':val) (m:mode) (x:var) (u:term),
+     Sem_eterm C (term_PatE (term_Val (val_E n v')) m n x u) C  (term_sub  u   x   v' ) 
+ | Sem_eterm_MapFoc : forall (C:ectxs) (t:term) (x:var) (t':term)
      (NotValt: term_NotVal t ),
-     Sem_eterm C (term_Map t x u)   (cons   (ectx_MapFoc x u)    C )   t
- | Sem_eterm_MapUnfoc : forall (C:ectxs) (x:var) (u:term) (v:val),
-     Sem_eterm   (cons   (ectx_MapFoc x u)    C )   (term_Val v) C (term_Map (term_Val v) x u)
- | Sem_eterm_MapRedAOpenFoc : forall (C:ectxs) (H:hdns) (v1 v2:val) (x:var) (u:term) (h':hdn)
+     Sem_eterm C (term_Map t x t')   (cons   (ectx_MapFoc x t')    C )   t
+ | Sem_eterm_MapUnfoc : forall (C:ectxs) (x:var) (t':term) (v:val),
+     Sem_eterm   (cons   (ectx_MapFoc x t')    C )   (term_Val v) C (term_Map (term_Val v) x t')
+ | Sem_eterm_MapRedAOpenFoc : forall (C:ectxs) (H:hdns) (v2 v1:val) (x:var) (t':term) (h':hdn)
      (hpMaxC: h' =  (hdns_max_hnames   (hdns_from_ectxs  C )  )  ),
-     Sem_eterm C (term_Map (term_Val (val_A H v1 v2)) x u)   (cons   (ectx_AOpenFoc  (hdns_incr_hnames  H   h' )   (val_incr_hnames  v1   h' ) )    C )    (term_sub  u   x    (val_incr_hnames  v2   h' )  ) 
- | Sem_eterm_AOpenUnfoc : forall (C:ectxs) (H:hdns) (v1 v2:val),
-     Sem_eterm   (cons  (ectx_AOpenFoc H v1)   C )   (term_Val v2) C (term_Val (val_A H v1 v2))
+     Sem_eterm C (term_Map (term_Val (val_A H v2 v1)) x t')   (cons   (ectx_AOpenFoc  (hdns_incr_hnames  H   h' )   (val_incr_hnames  v2   h' ) )    C )    (term_sub  t'   x    (val_incr_hnames  v1   h' )  ) 
+ | Sem_eterm_AOpenUnfoc : forall (C:ectxs) (H:hdns) (v2 v1:val),
+     Sem_eterm   (cons  (ectx_AOpenFoc H v2)   C )   (term_Val v1) C (term_Val (val_A H v2 v1))
  | Sem_eterm_AllocRed : forall (C:ectxs),
      Sem_eterm C term_Alloc C (term_Val (val_A  (hdns_from_list  (cons  1  nil) )  (val_D  1 ) (val_H  1 )))
- | Sem_eterm_ToAFoc : forall (C:ectxs) (t:term)
-     (NotValt: term_NotVal t ),
-     Sem_eterm C (term_ToA t)   (cons   ectx_ToAFoc    C )   t
- | Sem_eterm_ToAUnfoc : forall (C:ectxs) (v:val),
-     Sem_eterm   (cons   ectx_ToAFoc    C )   (term_Val v) C (term_ToA (term_Val v))
- | Sem_eterm_ToARed : forall (C:ectxs) (v:val),
-     Sem_eterm C (term_ToA (term_Val v)) C (term_Val (val_A  (hdns_from_list  nil )  v val_U))
+ | Sem_eterm_ToAFoc : forall (C:ectxs) (u:term)
+     (NotValu: term_NotVal u ),
+     Sem_eterm C (term_ToA u)   (cons   ectx_ToAFoc    C )   u
+ | Sem_eterm_ToAUnfoc : forall (C:ectxs) (v2:val),
+     Sem_eterm   (cons   ectx_ToAFoc    C )   (term_Val v2) C (term_ToA (term_Val v2))
+ | Sem_eterm_ToARed : forall (C:ectxs) (v2:val),
+     Sem_eterm C (term_ToA (term_Val v2)) C (term_Val (val_A  (hdns_from_list  nil )  v2 val_U))
  | Sem_eterm_FromAFoc : forall (C:ectxs) (t:term)
      (NotValt: term_NotVal t ),
      Sem_eterm C (term_FromA t)   (cons   ectx_FromAFoc    C )   t
  | Sem_eterm_FromAUnfoc : forall (C:ectxs) (v:val),
      Sem_eterm   (cons   ectx_FromAFoc    C )   (term_Val v) C (term_FromA (term_Val v))
- | Sem_eterm_FromARed : forall (C:ectxs) (v:val),
-     Sem_eterm C (term_FromA (term_Val (val_A  (hdns_from_list  nil )  v val_U))) C (term_Val v)
+ | Sem_eterm_FromARed : forall (C:ectxs) (v2:val),
+     Sem_eterm C (term_FromA (term_Val (val_A  (hdns_from_list  nil )  v2 val_U))) C (term_Val v2)
  | Sem_eterm_FillUFoc : forall (C:ectxs) (t:term)
      (NotValt: term_NotVal t ),
      Sem_eterm C (term_FillU t)   (cons   ectx_FillUFoc    C )   t
@@ -790,17 +790,18 @@ Inductive Sem_eterm : ectxs -> term -> ectxs -> term -> Prop :=    (* defn Sem_e
      Sem_eterm   (cons   (ectx_FillFFoc x m u)    C )   (term_Val v) C (term_FillF (term_Val v) x m u)
  | Sem_eterm_FillFRed : forall (C:ectxs) (h:hdn) (x:var) (m:mode) (u:term),
      Sem_eterm C (term_FillF (term_Val (val_D h)) x m u)  (ectxs_fill  C   h   (val_F x m u) )  (term_Val val_U)
- | Sem_eterm_FillCFoc1 : forall (C:ectxs) (t u:term)
+ | Sem_eterm_FillCFoc1 : forall (C:ectxs) (t t':term)
      (NotValt: term_NotVal t ),
-     Sem_eterm C (term_FillC t u)   (cons   (ectx_FillCFoc1 u)    C )   t
- | Sem_eterm_FillCUnfoc1 : forall (C:ectxs) (u:term) (v:val),
-     Sem_eterm   (cons   (ectx_FillCFoc1 u)    C )   (term_Val v) C (term_FillC (term_Val v) u)
- | Sem_eterm_FillCFoc2 : forall (C:ectxs) (v:val) (u:term),
-     Sem_eterm C (term_FillC (term_Val v) u)   (cons   (ectx_FillCFoc2 v)    C )   u
+     Sem_eterm C (term_FillC t t')   (cons   (ectx_FillCFoc1 t')    C )   t
+ | Sem_eterm_FillCUnfoc1 : forall (C:ectxs) (t':term) (v:val),
+     Sem_eterm   (cons   (ectx_FillCFoc1 t')    C )   (term_Val v) C (term_FillC (term_Val v) t')
+ | Sem_eterm_FillCFoc2 : forall (C:ectxs) (v:val) (t':term)
+     (NotValtp: term_NotVal t' ),
+     Sem_eterm C (term_FillC (term_Val v) t')   (cons   (ectx_FillCFoc2 v)    C )   t'
  | Sem_eterm_FillCUnfoc2 : forall (C:ectxs) (v v':val),
      Sem_eterm   (cons   (ectx_FillCFoc2 v)    C )   (term_Val v') C (term_FillC (term_Val v) (term_Val v'))
- | Sem_eterm_FillCRed : forall (C:ectxs) (h:hdn) (H:hdns) (v1 v2:val) (h':hdn)
+ | Sem_eterm_FillCRed : forall (C:ectxs) (h:hdn) (H:hdns) (v2 v1:val) (h':hdn)
      (hpMaxCh: h' =  (hdns_max_hnames   (HdnsM.union   (hdns_from_ectxs  C )     (hdns_from_list  (cons h nil) )  )  )  ),
-     Sem_eterm C (term_FillC (term_Val (val_D h)) (term_Val (val_A H v1 v2)))  (ectxs_fill  C   h    (val_incr_hnames  v1   h' )  )  (term_Val  (val_incr_hnames  v2   h' ) ).
+     Sem_eterm C (term_FillC (term_Val (val_D h)) (term_Val (val_A H v2 v1)))  (ectxs_fill  C   h    (val_incr_hnames  v2   h' )  )  (term_Val  (val_incr_hnames  v1   h' ) ).
 
 
