ott_coq/destination_calculus_proofs.v
@@ -61,18 +61,35 @@ Proof. Admitted.
 Lemma EmptyIsLinOnly : ctx_LinOnly ᴳ{}. (* TODO remove when we have actual definition of ctx_ValidOnly *)
 Proof. Admitted.
 
-Lemma EmptyUnionLeft : forall (G : ctx), G = G ⨄ ᴳ{}.
+Lemma EmptyUnionRight : forall (G : ctx), G = G ⨄ ᴳ{}.
 Proof. Admitted.
-Lemma EmptyUnionRight : forall (G : ctx), G = ᴳ{} ⨄ G.
+Lemma EmptyUnionLeft : forall (G : ctx), G = ᴳ{} ⨄ G.
 Proof. Admitted.
 
 Lemma DisjointDestOnlyVar : forall (G : ctx) (x : var) (m : mode) (T : type), ctx_DestOnly G -> ctx_Disjoint G (ᴳ{ x : m ‗ T}).
 Proof. Admitted.
 
+Lemma UnionCommutative : forall (G1 G2 : ctx), G1 ⨄ G2 = G2 ⨄ G1.
+Proof. Admitted.
+Lemma UnionAssociative : forall (G1 G2 G3 : ctx), G1 ⨄ (G2 ⨄ G3) = (G1 ⨄ G2) ⨄ G3.
+Proof. Admitted.
+
+Lemma StimesIsAction : forall (m n : mode) (G : ctx), m ᴳ· (n ᴳ· G) = (m · n) ᴳ· G.
+Proof. Admitted.
+
+Lemma TimesCommutative : forall (m n : mode), m · n = n · m.
+Proof. Admitted.
+Lemma TimesAssociative : forall (m1 m2 m3 : mode), m1 · (m2 · m3) = (m1 · m2) · m3.
+Proof. Admitted.
+Lemma TimesIdentityRight : forall (m : mode), m · ¹ν = m.
+Proof. Admitted.
+Lemma TimesIdentityLeft : forall (m : mode), ¹ν · m = m.
+Proof. Admitted.
+
 Ltac hauto_ctx :=
   hauto
     depth: 3
-    use: ValidOnlyUnionBackward, ValidOnlyUnionForward, ValidOnlyStimesEquiv, ValidOnlyMinusEquiv, DestOnlyUnionEquiv, DestOnlyStimesEquiv, LinNuOnlyUnionEquiv, LinNuOnlyStimesEquiv, LinOnlyUnionEquiv, LinOnlyStimesEquiv, LinNuOnlyWkLinOnly, LinOnlyWkValidOnly, IsLinNuWkIsLin, IsLinWkIsValid, DisjointStimesLeftEquiv, DisjointStimesRightEquiv, DisjointMinusLeftEquiv, DisjointMinusRightEquiv, DisjointNestedLeftEquiv, DisjointNestedRightEquiv, hdns_DisjointImpliesDisjoint, EmptyIsLinOnly, EmptyUnionLeft, EmptyUnionRight, DisjointDestOnlyVar.
+    use: ValidOnlyUnionBackward, ValidOnlyUnionForward, ValidOnlyStimesEquiv, ValidOnlyMinusEquiv, DestOnlyUnionEquiv, DestOnlyStimesEquiv, LinNuOnlyUnionEquiv, LinNuOnlyStimesEquiv, LinOnlyUnionEquiv, LinOnlyStimesEquiv, LinNuOnlyWkLinOnly, LinOnlyWkValidOnly, IsLinNuWkIsLin, IsLinWkIsValid, DisjointStimesLeftEquiv, DisjointStimesRightEquiv, DisjointMinusLeftEquiv, DisjointMinusRightEquiv, DisjointNestedLeftEquiv, DisjointNestedRightEquiv, hdns_DisjointImpliesDisjoint, EmptyIsLinOnly, EmptyUnionLeft, EmptyUnionRight, DisjointDestOnlyVar, UnionCommutative, UnionAssociative, StimesIsAction, TimesCommutative, TimesAssociative, TimesIdentityRight, TimesIdentityLeft.
 
 Lemma Ty_ectxs_LinOnlyD : forall (D : ctx) (C : ectxs) (T U0 : type) (TyC: D ⊣ C : T ↣ U0), ctx_LinOnly D.
 Proof.
@@ -95,13 +112,22 @@ Proof.
   - hauto_ctx.
   - hauto_ctx.
   - hauto_ctx.
-  - assert (ctx_LinOnly (¹↑ ᴳ· D2)) by (hauto l: on use: LinOnlyUnionEquiv, LinOnlyStimesEquiv, (mode_IsLinProof (Fin 1))).
-    assert (ctx_Disjoint (D1 ⨄ D2) (ᴳ-D3)) by (apply (hdns_DisjointImpliesDisjoint (D1 ⨄ D2) (ᴳ-D3) C (T1 ⧔ U) U0); tauto).
-    assert (ctx_Disjoint (¹↑ ᴳ· D2) D3) by (sblast use: DisjointNestedLeftEquiv, DisjointMinusRightEquiv, DisjointStimesLeftEquiv).
-    rewrite (LinOnlyUnionEquiv (¹↑ ᴳ· D2) D3). split; tauto.
+  - assert (ctx_LinOnly (¹↑ ᴳ· D1)).
+      { hauto l: on use: LinOnlyUnionEquiv, LinOnlyStimesEquiv, (mode_IsLinProof (Fin 1)). }
+    assert (ctx_Disjoint (D1 ⨄ D2) (ᴳ-D3)).
+      { apply (hdns_DisjointImpliesDisjoint (D1 ⨄ D2) (ᴳ-D3) C (U ⧔ T') U0); tauto. }
+    assert (ctx_Disjoint (¹↑ ᴳ· D1) D3).
+      { sblast use: DisjointNestedLeftEquiv, DisjointMinusRightEquiv, DisjointStimesLeftEquiv. }
+    rewrite (LinOnlyUnionEquiv (¹↑ ᴳ· D1) D3). split; tauto.
 Qed.
 
-Lemma tSubLemma : forall (D1 D2 : ctx) (m : mode) (T1 T2 : type) (t' : term) (x : var) (v : val), ctx_DestOnly D2 -> (D2 ⨄ ᴳ{ x : m ‗ T1} ⊢ t' : T2) -> (D1 ⊢ ᵥ₎ v : T1) -> (m ᴳ· D1 ⨄ D2 ⊢ t' ᵗ[ x ≔ v] : T2). Proof. Admitted.
+Lemma tSubLemma : forall (D1 D2 : ctx) (m : mode) (T U : type) (u : term) (x : var) (v : val), ctx_DestOnly D1 -> ctx_DestOnly D2 -> (D2 ⨄ ᴳ{ x : m ‗ T} ⊢ u : U) -> (D1 ⊢ ᵥ₎ v : T) -> (m ᴳ· D1 ⨄ D2 ⊢ u ᵗ[ x ≔ v] : U).
+Proof. Admitted.
+
+Lemma tSubLemma2 : forall (D11 D12 D2 : ctx) (m : mode) (T1 T2 U : type) (u : term) (x1 x2 : var) (v1 v2 : val), ctx_DestOnly D11 -> ctx_DestOnly D12 -> ctx_DestOnly D2 -> (ctx_Disjoint ᴳ{ x1 : m ‗ T1} ᴳ{ x2 : m ‗ T2}) -> (D2 ⨄ ᴳ{ x1 : m ‗ T1} ⨄ ᴳ{ x2 : m ‗ T2} ⊢ u : U) -> (D11 ⊢ ᵥ₎ v1 : T1) -> (D12 ⊢ ᵥ₎ v2 : T2) -> (m ᴳ· (D11 ⨄ D12) ⨄ D2 ⊢ u ᵗ[ x1 ≔ v1 ] ᵗ[ x2 ≔ v2 ] : U).
+Proof. Admitted.
+
+(* TODO: bump only internal names of ampar *)
 
 Theorem Preservation : forall (C C' : ectxs) (t t' : term) (T : type), ⊢ C ʲ[t] : T /\
   C ʲ[t] ⟶ C' ʲ[t'] -> ⊢ C' ʲ[t'] : T.
@@ -109,90 +135,168 @@ Proof.
     intros C C' t t' T (Tyj & Redj). destruct Tyj. destruct Redj.
     - (* Sem-eterm-AppFoc1 *)
       inversion Tyt; subst.
-      rename Tyt into TyApp, Tyt0 into Tyt, P1 into D1, P2 into D2, T into T2.
-      assert (ctx_LinOnly (m ᴳ· D1 ⨄ D2)) as LinOnlyD by (apply (Ty_ectxs_LinOnlyD (m ᴳ· D1 ⨄ D2) C T2 U0); tauto).
-      constructor 1 with (D := D1) (T := T1) (t := t); swap 1 3. constructor 2 with (D2 := D2) (m := m) (u := u) (T2 := T2).
+      rename Tyt into TyApp, Tyt0 into Tyt, P1 into D1, P2 into D2, T into U, T0 into T.
+      assert (ctx_LinOnly (m ᴳ· D1 ⨄ D2)) as LinOnlyD.
+        { apply (Ty_ectxs_LinOnlyD (m ᴳ· D1 ⨄ D2) C U U0); tauto. }
+      constructor 1 with (D := D1) (T := T) (t := t); swap 1 3. constructor 2 with (D2 := D2) (m := m) (t' := t') (U := U).
       all: hauto_ctx.
     - (* Sem-eterm-AppUnfoc1 *)
-      inversion Tyt; subst. rename H2 into TyRv, TyC into TyCc, D into D1, ValidOnlyD into ValidOnlyD1, DestOnlyD into DestOnlyD1. clear H0.
-      inversion TyCc; subst. clear DestOnlyD0. rename T into T1.
-      assert (ctx_LinOnly (m ᴳ· D1 ⨄ D2)) as LinOnlyD by (apply (Ty_ectxs_LinOnlyD (m ᴳ· D1 ⨄ D2) C T2 U0); tauto).
-      assert (m ᴳ· D1 ⨄ D2 ⊢ ᵥ₎ v ≻ u : T2) as TyApp by (apply (Ty_term_App m D1 D2 (ᵥ₎ v) u T2 T1); tauto).
-      constructor 1 with (D := (m ᴳ· D1 ⨄ D2)) (T := T2) (t := ᵥ₎ v ≻ u). all: hauto_ctx.
+      inversion Tyt; subst. rename TyC into TyCc, D into D1, ValidOnlyD into ValidOnlyD1, DestOnlyD into DestOnlyD1. clear H1.
+      inversion TyCc; subst. clear DestOnlyD0.
+      assert (ctx_LinOnly (m ᴳ· D1 ⨄ D2)) as LinOnlyD.
+        { apply (Ty_ectxs_LinOnlyD (m ᴳ· D1 ⨄ D2) C U U0); tauto. }
+      assert (m ᴳ· D1 ⨄ D2 ⊢ ᵥ₎ v ≻ t' : U) as TyApp.
+        { apply (Ty_term_App m D1 D2 (ᵥ₎ v) t' U T); tauto. }
+      constructor 1 with (D := (m ᴳ· D1 ⨄ D2)) (T := U) (t := ᵥ₎ v ≻ t'). all: hauto_ctx.
     - (* Sem-eterm-AppFoc2 *)
       inversion Tyt; subst.
-      rename Tyt into TyApp, Tyt0 into Tyt, P1 into D1, P2 into D2, T into T2.
-      assert (ctx_LinOnly (m ᴳ· D1 ⨄ D2)) as LinOnlyD by (apply (Ty_ectxs_LinOnlyD (m ᴳ· D1 ⨄ D2) C T2 U0); tauto).
-      constructor 1 with (D := D2) (T := T1 ⁔ m → T2) (t := u); swap 1 3. constructor 3 with (D1 := D1) (m := m) (v := v) (T1 := T1) (T2 := T2). all: hauto_ctx.
+      rename Tyt into TyApp, Tyt0 into Tyt, P1 into D1, P2 into D2, T into U, T0 into T.
+      assert (ctx_LinOnly (m ᴳ· D1 ⨄ D2)) as LinOnlyD.
+        { apply (Ty_ectxs_LinOnlyD (m ᴳ· D1 ⨄ D2) C U U0); tauto. }
+      constructor 1 with (D := D2) (T := T ⁔ m → U) (t := t'); swap 1 3. constructor 3 with (D1 := D1) (m := m) (v := v) (T := T) (U := U). all: hauto_ctx.
     - (* Sem-eterm-AppUnfoc2 *)
-      inversion Tyt; subst. rename H2 into TyRv, TyC into TyCc, D into D2, ValidOnlyD into ValidOnlyD2, DestOnlyD into DestOnlyD2. clear H0.
-      inversion TyCc; subst. clear DestOnlyD0. rename Tyt into Tyu, Tyv into Tyt.
-      assert (m ᴳ· D1 ⨄ D2 ⊢ ᵥ₎ v ≻ ᵥ₎ v' : T2) as TyApp by (apply (Ty_term_App m D1 D2 (ᵥ₎ v) (ᵥ₎ v') T2 T1); tauto).
-      assert (ctx_LinOnly (m ᴳ· D1 ⨄ D2)) as LinOnlyD by (apply (Ty_ectxs_LinOnlyD (m ᴳ· D1 ⨄ D2) C T2 U0); tauto).
-      constructor 1 with (D := (m ᴳ· D1 ⨄ D2)) (T := T2) (t := (ᵥ₎ v) ≻ (ᵥ₎ v')). all: hauto_ctx.
+      inversion Tyt; subst. rename TyRv into TyRvp, TyC into TyCc, D into D2, ValidOnlyD into ValidOnlyD2, DestOnlyD into DestOnlyD2. clear H1.
+      inversion TyCc; subst. clear DestOnlyD0. rename Tyt into Tytp, Tyv into Tyt, T0 into T.
+      assert (m ᴳ· D1 ⨄ D2 ⊢ ᵥ₎ v ≻ ᵥ₎ v' : U) as TyApp.
+        { apply (Ty_term_App m D1 D2 (ᵥ₎ v) (ᵥ₎ v') U T); tauto. }
+      assert (ctx_LinOnly (m ᴳ· D1 ⨄ D2)) as LinOnlyD.
+        { apply (Ty_ectxs_LinOnlyD (m ᴳ· D1 ⨄ D2) C U U0); tauto. }
+      constructor 1 with (D := (m ᴳ· D1 ⨄ D2)) (T := U) (t := (ᵥ₎ v) ≻ (ᵥ₎ v')). all: hauto_ctx.
     - (* Sem-eterm-AppRed *)
       inversion Tyt; subst.
-      assert (m = m0) as Eqmm0 by (inversion_clear Tyu; inversion_clear H0; tauto).
-      rewrite <- Eqmm0 in Tyu, Tyt, TyC, DestOnlyD, ValidOnlyD. clear Eqmm0. clear m0. rename P1 into D1, P2 into D2. rename Tyt into TyApp, Tyt0 into Tyt, T into T2, t into t'.
-      inversion Tyu; subst. clear H0. rename H2 into TyRv'.
-      inversion TyRv'; subst. rename Tyt0 into Tyt'. rename H1 into DestOnlyD2.
-      assert (m ᴳ· D1 ⨄ D2 ⊢ t' ᵗ[ x ≔ v] : T2) as Tytpsub by (apply (tSubLemma D1 D2 m T1 T2 t' x v); tauto).
-      constructor 1 with (D := (m ᴳ· D1 ⨄ D2)) (T := T2) (t := t' ᵗ[ x ≔ v]). all: hauto_ctx.
+      assert (m = m0) as Eqmm0.
+        { inversion_clear Tytp; inversion_clear TyRv; tauto. }
+      rewrite <- Eqmm0 in Tyt, Tytp, TyC, DestOnlyD, ValidOnlyD. clear Eqmm0. clear m0. rename P1 into D1, P2 into D2. rename Tyt into TyApp, Tyt0 into Tyt, T into U, T0 into T.
+      inversion Tytp; subst. clear H1. rename TyRv into TyRv'.
+      inversion TyRv'; subst. rename H1 into DestOnlyD2.
+      assert (m ᴳ· D1 ⨄ D2 ⊢ u ᵗ[ x ≔ v] : U) as Tyusub.
+        { apply (tSubLemma D1 D2 m T U u x v); hauto_ctx. }
+      constructor 1 with (D := (m ᴳ· D1 ⨄ D2)) (T := U) (t := u ᵗ[ x ≔ v]). all: hauto_ctx.
     - (* Sem-eterm-PatUFoc *)
       inversion Tyt; subst.
       rename Tyt into TyPat, Tyt0 into Tyt, P1 into D1, P2 into D2, T into T2.
-      assert (ctx_LinOnly (D1 ⨄ D2)) as LinOnlyD by (apply (Ty_ectxs_LinOnlyD (D1 ⨄ D2) C T2 U0); tauto).
+      assert (ctx_LinOnly (D1 ⨄ D2)) as LinOnlyD.
+        { apply (Ty_ectxs_LinOnlyD (D1 ⨄ D2) C T2 U0); tauto. }
       constructor 1 with (D := D1) (T := 𝟏) (t := t); swap 1 3. constructor 4 with (D2 := D2) (U := T2) (u := u). all: hauto_ctx.
     - (* Sem-eterm-PatUUnfoc *)
-      inversion Tyt; subst. rename H2 into TyRv, TyC into TyCc, D into D1, ValidOnlyD into ValidOnlyD1, DestOnlyD into DestOnlyD1. clear H0.
+      inversion Tyt; subst. rename TyC into TyCc, D into D1, ValidOnlyD into ValidOnlyD1, DestOnlyD into DestOnlyD1. clear H1.
       inversion TyCc; subst. clear DestOnlyD0. rename U into T2.
-      assert (ctx_LinOnly (D1 ⨄ D2)) as LinOnlyD by (apply (Ty_ectxs_LinOnlyD (D1 ⨄ D2) C T2 U0); tauto).
-      assert (D1 ⨄ D2 ⊢ ᵥ₎ v ᵗ; u : T2) as TyPat by (apply (Ty_term_PatU D1 D2 (ᵥ₎ v) u T2); tauto).
+      assert (ctx_LinOnly (D1 ⨄ D2)) as LinOnlyD.
+        { apply (Ty_ectxs_LinOnlyD (D1 ⨄ D2) C T2 U0); tauto. }
+      assert (D1 ⨄ D2 ⊢ ᵥ₎ v ᵗ; u : T2) as TyPat.
+        { apply (Ty_term_PatU D1 D2 (ᵥ₎ v) u T2); tauto. }
       constructor 1 with (D := (D1 ⨄ D2)) (T := T2) (t := ᵥ₎ v ᵗ; u). all: hauto_ctx.
     - (* Sem-eterm-PatURed *)
       inversion Tyt; subst.
       rename P1 into D1, P2 into D2. rename Tyt into TyPat, Tyt0 into Tyt, T into T2.
-      inversion Tyt; subst. rename H0 into DestOnlyD1, H2 into TyRv.
+      inversion Tyt; subst. rename H1 into DestOnlyD1.
       inversion TyRv; subst.
       constructor 1 with (D := D2) (T := T2) (t := u). all: hauto_ctx.
     - (* Sem-eterm-PatSFoc *)
       inversion Tyt; subst.
       rename Tyt into TyPat, Tyt0 into Tyt, P1 into D1, P2 into D2, T into U.
-      assert (ctx_LinOnly (m ᴳ· D1 ⨄ D2)) as LinOnlyD by (apply (Ty_ectxs_LinOnlyD (m ᴳ· D1 ⨄ D2) C U U0); tauto).
+      assert (ctx_LinOnly (m ᴳ· D1 ⨄ D2)) as LinOnlyD.
+        { apply (Ty_ectxs_LinOnlyD (m ᴳ· D1 ⨄ D2) C U U0); tauto. }
       constructor 1 with (D := D1) (T := (T1 ⨁ T2)) (t := t) ; swap 1 3. constructor 5 with (D1 := D1) (D2 := D2) (m := m) (u1 := u1) (x1 := x1) (u2 := u2) (x2 := x2) (U := U). all: hauto_ctx.
     - (* Sem-eterm-PatSUnfoc *)
-      inversion Tyt; subst. rename H2 into TyRv, TyC into TyCc, D into D1, ValidOnlyD into ValidOnlyD1, DestOnlyD into DestOnlyD1. clear H0.
+      inversion Tyt; subst. rename TyC into TyCc, D into D1, ValidOnlyD into ValidOnlyD1, DestOnlyD into DestOnlyD1. clear H1.
       inversion TyCc; subst. clear DestOnlyD0.
-      assert (ctx_LinOnly (m ᴳ· D1 ⨄ D2)) as LinOnlyD by (apply (Ty_ectxs_LinOnlyD (m ᴳ· D1 ⨄ D2) C U U0); tauto).
-      assert (m ᴳ· D1 ⨄ D2 ⊢ ᵥ₎ v ≻caseˢ m {Inl x1 ⟼ u1, Inr x2 ⟼ u2} : U) as TyPat by (apply (Ty_term_PatS m D1 D2 (ᵥ₎ v) x1 u1 x2 u2 U T1 T2); hauto_ctx).
+      assert (ctx_LinOnly (m ᴳ· D1 ⨄ D2)) as LinOnlyD.
+        { apply (Ty_ectxs_LinOnlyD (m ᴳ· D1 ⨄ D2) C U U0); tauto. }
+      assert (m ᴳ· D1 ⨄ D2 ⊢ ᵥ₎ v ≻caseˢ m {Inl x1 ⟼ u1, Inr x2 ⟼ u2} : U) as TyPat.
+        { apply (Ty_term_PatS m D1 D2 (ᵥ₎ v) x1 u1 x2 u2 U T1 T2); hauto_ctx. }
       constructor 1 with (D := (m ᴳ· D1 ⨄ D2)) (T := U) (t := ᵥ₎ v ≻caseˢ m {Inl x1 ⟼ u1, Inr x2 ⟼ u2}). all: hauto_ctx.
     - (* Sem-eterm-PatLRed *)
       inversion Tyt; subst.
       rename P1 into D1, P2 into D2. rename Tyt into TyPat, Tyt0 into Tyt, T into U.
-      inversion Tyt; subst. rename H0 into DestOnlyD1, H2 into TyRInlv.
-      inversion TyRInlv; subst.
-      assert (D1 ⊢ ᵥ₎ v : T1) as Tyt' by (apply Ty_term_Val; tauto).
-      assert (m ᴳ· D1 ⨄ D2 ⊢ u1 ᵗ[ x1 ≔ v] : U) as Tyusub by (apply (tSubLemma D1 D2 m T1 U u1 x1 v); hauto_ctx).
-      constructor 1 with (D := (m ᴳ· D1 ⨄ D2)) (T := U) (t := u1 ᵗ[ x1 ≔ v]). all: hauto_ctx.
+      inversion Tyt; subst. rename H1 into DestOnlyD1, TyRv into TyRInlv1.
+      inversion TyRInlv1; subst.
+      assert (D1 ⊢ ᵥ₎ v1 : T1) as Tyt'.
+        { apply Ty_term_Val; tauto. }
+      assert (m ᴳ· D1 ⨄ D2 ⊢ u1 ᵗ[ x1 ≔ v1] : U) as Tyusub.
+        { apply (tSubLemma D1 D2 m T1 U u1 x1 v1); hauto_ctx. }
+      constructor 1 with (D := (m ᴳ· D1 ⨄ D2)) (T := U) (t := u1 ᵗ[ x1 ≔ v1]). all: hauto_ctx.
     - (* Sem-eterm-PatRRed *)
       inversion Tyt; subst.
       rename P1 into D1, P2 into D2. rename Tyt into TyPat, Tyt0 into Tyt, T into U.
-      inversion Tyt; subst. rename H0 into DestOnlyD1, H2 into TyRInlv.
-      inversion TyRInlv; subst.
-      assert (D1 ⊢ ᵥ₎ v : T2) as Tyt' by (apply Ty_term_Val; tauto).
-      assert (m ᴳ· D1 ⨄ D2 ⊢ u2 ᵗ[ x2 ≔ v] : U) as Tyusub by (apply (tSubLemma D1 D2 m T2 U u2 x2 v); hauto_ctx).
-      constructor 1 with (D := (m ᴳ· D1 ⨄ D2)) (T := U) (t := u2 ᵗ[ x2 ≔ v]). all: hauto_ctx.
+      inversion Tyt; subst. rename H1 into DestOnlyD1, TyRv into TyRInlv2.
+      inversion TyRInlv2; subst.
+      assert (D1 ⊢ ᵥ₎ v2 : T2) as Tyt'.
+        { apply Ty_term_Val; tauto. }
+      assert (m ᴳ· D1 ⨄ D2 ⊢ u2 ᵗ[ x2 ≔ v2] : U) as Tyusub.
+        { apply (tSubLemma D1 D2 m T2 U u2 x2 v2); hauto_ctx. }
+      constructor 1 with (D := (m ᴳ· D1 ⨄ D2)) (T := U) (t := u2 ᵗ[ x2 ≔ v2]). all: hauto_ctx.
     - (* Sem-eterm-PatPFoc *)
       inversion Tyt; subst.
       rename Tyt into TyPat, Tyt0 into Tyt, P1 into D1, P2 into D2, T into U.
-      assert (ctx_LinOnly (m ᴳ· D1 ⨄ D2)) as LinOnlyD by (apply (Ty_ectxs_LinOnlyD (m ᴳ· D1 ⨄ D2) C U U0); tauto).
+      assert (ctx_LinOnly (m ᴳ· D1 ⨄ D2)) as LinOnlyD.
+        { apply (Ty_ectxs_LinOnlyD (m ᴳ· D1 ⨄ D2) C U U0); tauto. }
       constructor 1 with (D := D1) (T := (T1 ⨂ T2)) (t := t) ; swap 1 3. constructor 6 with (D1 := D1) (D2 := D2) (u := u) (x1 := x1) (x2 := x2) (U := U). all: hauto_ctx.
     - (* Sem-eterm-PatPUnfoc *)
-      inversion Tyt; subst. rename H2 into TyRv, TyC into TyCc, D into D1, ValidOnlyD into ValidOnlyD1, DestOnlyD into DestOnlyD1. clear H0.
+      inversion Tyt; subst. rename TyC into TyCc, D into D1, ValidOnlyD into ValidOnlyD1, DestOnlyD into DestOnlyD1. clear H1.
       inversion TyCc; subst. clear DestOnlyD0.
-      assert (ctx_LinOnly (m ᴳ· D1 ⨄ D2)) as LinOnlyD by (apply (Ty_ectxs_LinOnlyD (m ᴳ· D1 ⨄ D2) C U U0); tauto).
-      assert (m ᴳ· D1 ⨄ D2 ⊢ ᵥ₎ v ≻caseᵖ m ᵗ(x1 , x2) ⟼ u : U) as TyPat by (apply (Ty_term_PatP m D1 D2 (ᵥ₎ v) x1 x2 u U T1 T2); hauto_ctx).
+      assert (ctx_LinOnly (m ᴳ· D1 ⨄ D2)) as LinOnlyD.
+        { apply (Ty_ectxs_LinOnlyD (m ᴳ· D1 ⨄ D2) C U U0); tauto. }
+      assert (m ᴳ· D1 ⨄ D2 ⊢ ᵥ₎ v ≻caseᵖ m ᵗ(x1 , x2) ⟼ u : U) as TyPat.
+        { apply (Ty_term_PatP m D1 D2 (ᵥ₎ v) x1 x2 u U T1 T2); hauto_ctx. }
       constructor 1 with (D := (m ᴳ· D1 ⨄ D2)) (T := U) (t := ᵥ₎ v ≻caseᵖ m ᵗ(x1 , x2) ⟼ u). all: hauto_ctx.
+    - (* Sem-eterm-PatPRed *)
+      inversion Tyt; subst.
+      rename P1 into D1, P2 into D2. rename Tyt into TyPat, Tyt0 into Tyt, T into U.
+      inversion Tyt; subst. rename H1 into DestOnlyD1.
+      inversion TyRv; subst. rename G1 into D11, G2 into D12.
+      assert (D11 ⊢ ᵥ₎ v1 : T1) as Tyt1.
+        { apply Ty_term_Val; hauto_ctx. }
+      assert (D12 ⊢ ᵥ₎ v2 : T2) as Tyt2.
+        { apply Ty_term_Val; hauto_ctx. }
+      assert (m ᴳ· (D11 ⨄ D12) ⨄ D2 ⊢ u ᵗ[ x1 ≔ v1] ᵗ[ x2 ≔ v2] : U) as Tyusub.
+        { apply (tSubLemma2 D11 D12 D2 m T1 T2 U u x1 x2 v1 v2); hauto_ctx. }
+      constructor 1 with (D := (m ᴳ· (D11 ⨄ D12) ⨄ D2)) (T := U) (t := u ᵗ[ x1 ≔ v1] ᵗ[ x2 ≔ v2]). all: hauto_ctx.
+    - (* Sem-eterm-PatEFoc *)
+      inversion Tyt; subst.
+      rename Tyt into TyPat, Tyt0 into Tyt, P1 into D1, P2 into D2, T into U, T0 into T.
+      assert (ctx_LinOnly (m ᴳ· D1 ⨄ D2)) as LinOnlyD.
+        { apply (Ty_ectxs_LinOnlyD (m ᴳ· D1 ⨄ D2) C U U0); tauto. }
+      constructor 1 with (D := D1) (T := (! n ⁔ T)) (t := t) ; swap 1 3. constructor 7 with (D1 := D1) (D2 := D2) (u := u) (x := x) (U := U). all: hauto_ctx.
+    - (* Sem-eterm-PatEUnfoc *)
+      inversion Tyt; subst. rename TyC into TyCc, D into D1, ValidOnlyD into ValidOnlyD1, DestOnlyD into DestOnlyD1. clear H1.
+      inversion TyCc; subst. clear DestOnlyD0. rename T0 into T.
+      assert (ctx_LinOnly (m ᴳ· D1 ⨄ D2)) as LinOnlyD.
+        { apply (Ty_ectxs_LinOnlyD (m ᴳ· D1 ⨄ D2) C U U0); tauto. }
+      assert (m ᴳ· D1 ⨄ D2 ⊢ ᵥ₎ v ≻caseᵉ m ᴇ n ⁔ x ⟼ u : U) as TyPat.
+        { apply (Ty_term_PatE m D1 D2 (ᵥ₎ v) n x u U T); hauto_ctx. }
+      constructor 1 with (D := (m ᴳ· D1 ⨄ D2)) (T := U) (t := ᵥ₎ v ≻caseᵉ m ᴇ n ⁔ x ⟼ u). all: hauto_ctx.
+    - (* Sem-eterm-PatERed *)
+      inversion Tyt; subst.
+      rename P1 into D1, P2 into D2. rename Tyt into TyPat, Tyt0 into Tyt, T into U, T0 into T.
+      inversion Tyt; subst. rename H1 into DestOnlyD1.
+      inversion TyRv; subst.
+      assert (G ⊢ ᵥ₎ v' : T) as Tyt'.
+        { apply Ty_term_Val; hauto_ctx. }
+      assert ((m · n) ᴳ· G ⨄ D2 ⊢ u ᵗ[ x ≔ v'] : U) as Tyusub.
+        { apply (tSubLemma G D2 (m · n) T U u x v'). all: try hauto_ctx. }
+      constructor 1 with (D := (m ᴳ· (n ᴳ· G) ⨄ D2)) (T := U) (t := u ᵗ[ x ≔ v']). all: hauto_ctx.
+    - (* Sem-eterm-MapFoc *)
+      inversion Tyt; subst. rename T0 into T.
+      rename Tyt into TyMap, Tyt0 into Tyt, P1 into D1, P2 into D2.
+      assert (ctx_LinOnly (D1 ⨄ D2)) as LinOnlyD.
+        { apply (Ty_ectxs_LinOnlyD (D1 ⨄ D2) C (U ⧔ T') U0); tauto. }
+      constructor 1 with (D := D1) (T := U ⧔ T) (t := t); swap 1 3. constructor 8 with (D1 := D1) (D2 := D2) (t' := t') (x := x) (T := T) (T' := T') (U := U). all: hauto_ctx.
+    - (* Sem-eterm-MapUnfoc *)
+      inversion Tyt; subst. rename TyC into TyCc, D into D1, ValidOnlyD into ValidOnlyD1, DestOnlyD into DestOnlyD1. clear H1.
+      inversion TyCc; subst. clear DestOnlyD0. rename T0 into T.
+      assert (ctx_LinOnly (D1 ⨄ D2)) as LinOnlyD.
+        { apply (Ty_ectxs_LinOnlyD (D1 ⨄ D2) C (U ⧔ T') U0); tauto. }
+      assert (D1 ⨄ D2 ⊢ ᵥ₎ v ≻map x ⟼ t' : U ⧔ T') as TyMap.
+        { apply (Ty_term_Map D1 D2 (ᵥ₎ v) x t' U T' T); hauto_ctx. }
+      constructor 1 with (D := (D1 ⨄ D2)) (T := U ⧔ T') (t := ᵥ₎ v ≻map x ⟼ t'). all: hauto_ctx.
+    - (* Sem-eterm-MapRedAOpenFoc *)
+      inversion Tyt; subst.
+      rename P1 into D1, P2 into D2. rename Tyt into TyMap, Tyt0 into Tyt, T0 into T.
+      inversion Tyt; subst. rename H2 into DestOnlyD1.
+      assert (D1 ⊢ ᵥ₎ H ⟨ v2 ❟ v1 ⟩ : U ⧔ T) as Tyt'.
+        { apply Ty_term_Val; hauto_ctx. }
+      admit.
     - give_up.
 Admitted.
 
